Cartouches

SPA.thy
@@ -11,200 +11,200 @@ section \<open>Syntax of First-Order Logic\<close>
 
 type_synonym id = String.literal
 
-datatype tm = Var id | Fun id "tm list"
+datatype tm = Var id | Fun id \<open>tm list\<close>
 
-datatype fm = Truth | Falsity | Pre id "tm list" | Imp fm fm | Iff fm fm | Con fm fm | Dis fm fm |
+datatype fm = Truth | Falsity | Pre id \<open>tm list\<close> | Imp fm fm | Iff fm fm | Con fm fm | Dis fm fm |
   Neg fm | Exi id fm | Uni id fm
 
 section \<open>Definition of Rules and Axioms on Formulas\<close>
 
-abbreviation (input) "fail \<equiv> Truth"
+abbreviation (input) \<open>fail \<equiv> Truth\<close>
 
-definition zip_eq :: "tm list \<Rightarrow> tm list \<Rightarrow> fm list"
+definition zip_eq :: \<open>tm list \<Rightarrow> tm list \<Rightarrow> fm list\<close>
   where
-    "zip_eq l l' \<equiv> map (\<lambda>(t, t'). Pre (STR ''='') [t, t']) (zip l l')"
+    \<open>zip_eq l l' \<equiv> map (\<lambda>(t, t'). Pre (STR ''='') [t, t']) (zip l l')\<close>
 
-primrec occurs_in :: "id \<Rightarrow> tm \<Rightarrow> bool" and occurs_in_list :: "id \<Rightarrow> tm list \<Rightarrow> bool"
+primrec occurs_in :: \<open>id \<Rightarrow> tm \<Rightarrow> bool\<close> and occurs_in_list :: \<open>id \<Rightarrow> tm list \<Rightarrow> bool\<close>
   where
-    "occurs_in i (Var x) = (i = x)" |
-    "occurs_in i (Fun _ l) = occurs_in_list i l" |
-    "occurs_in_list _ [] = False" |
-    "occurs_in_list i (h # t) = (occurs_in i h \<or> occurs_in_list i t)"
+    \<open>occurs_in i (Var x) = (i = x)\<close> |
+    \<open>occurs_in i (Fun _ l) = occurs_in_list i l\<close> |
+    \<open>occurs_in_list _ [] = False\<close> |
+    \<open>occurs_in_list i (h # t) = (occurs_in i h \<or> occurs_in_list i t)\<close>
 
-primrec free_in :: "id \<Rightarrow> fm \<Rightarrow> bool"
+primrec free_in :: \<open>id \<Rightarrow> fm \<Rightarrow> bool\<close>
   where
-    "free_in _ Truth = False" |
-    "free_in _ Falsity = False" |
-    "free_in i (Pre _ l) = occurs_in_list i l" |
-    "free_in i (Imp p q) = (free_in i p \<or> free_in i q)" |
-    "free_in i (Iff p q) = (free_in i p \<or> free_in i q)" |
-    "free_in i (Con p q) = (free_in i p \<or> free_in i q)" |
-    "free_in i (Dis p q) = (free_in i p \<or> free_in i q)" |
-    "free_in i (Neg p) = free_in i p" |
-    "free_in i (Exi x p) = (i \<noteq> x \<and> free_in i p)" |
-    "free_in i (Uni x p) = (i \<noteq> x \<and> free_in i p)"
+    \<open>free_in _ Truth = False\<close> |
+    \<open>free_in _ Falsity = False\<close> |
+    \<open>free_in i (Pre _ l) = occurs_in_list i l\<close> |
+    \<open>free_in i (Imp p q) = (free_in i p \<or> free_in i q)\<close> |
+    \<open>free_in i (Iff p q) = (free_in i p \<or> free_in i q)\<close> |
+    \<open>free_in i (Con p q) = (free_in i p \<or> free_in i q)\<close> |
+    \<open>free_in i (Dis p q) = (free_in i p \<or> free_in i q)\<close> |
+    \<open>free_in i (Neg p) = free_in i p\<close> |
+    \<open>free_in i (Exi x p) = (i \<noteq> x \<and> free_in i p)\<close> |
+    \<open>free_in i (Uni x p) = (i \<noteq> x \<and> free_in i p)\<close>
 
-primrec equal_length :: "tm list \<Rightarrow> tm list \<Rightarrow> bool"
+primrec equal_length :: \<open>tm list \<Rightarrow> tm list \<Rightarrow> bool\<close>
   where
-    "equal_length l [] = (case l of [] \<Rightarrow> True | _ # _ \<Rightarrow> False)" |
-    "equal_length l (_ # r') = (case l of [] \<Rightarrow> False | _ # l' \<Rightarrow> equal_length l' r')"
+    \<open>equal_length l [] = (case l of [] \<Rightarrow> True | _ # _ \<Rightarrow> False)\<close> |
+    \<open>equal_length l (_ # r') = (case l of [] \<Rightarrow> False | _ # l' \<Rightarrow> equal_length l' r')\<close>
 
-abbreviation (input) "chain l l' p \<equiv> if equal_length l l' then foldr Imp (zip_eq l l') p else fail"
+abbreviation (input) \<open>chain l l' p \<equiv> if equal_length l l' then foldr Imp (zip_eq l l') p else fail\<close>
 
-definition modusponens' :: "fm \<Rightarrow> fm \<Rightarrow> fm"
+definition modusponens' :: \<open>fm \<Rightarrow> fm \<Rightarrow> fm\<close>
   where
-    "modusponens' s s' \<equiv> case s of Imp p q \<Rightarrow> let p' = s' in if p = p' then q else fail | _ \<Rightarrow> fail"
+    \<open>modusponens' s s' \<equiv> case s of Imp p q \<Rightarrow> let p' = s' in if p = p' then q else fail | _ \<Rightarrow> fail\<close>
 
-definition gen' :: "id \<Rightarrow> fm \<Rightarrow> fm"
+definition gen' :: \<open>id \<Rightarrow> fm \<Rightarrow> fm\<close>
   where
-    "gen' x s \<equiv> Uni x s"
+    \<open>gen' x s \<equiv> Uni x s\<close>
 
-definition axiom_addimp' :: "fm \<Rightarrow> fm \<Rightarrow> fm"
+definition axiom_addimp' :: \<open>fm \<Rightarrow> fm \<Rightarrow> fm\<close>
   where
-    "axiom_addimp' p q \<equiv> Imp p (Imp q p)"
+    \<open>axiom_addimp' p q \<equiv> Imp p (Imp q p)\<close>
 
-definition axiom_distribimp' :: "fm \<Rightarrow> fm \<Rightarrow> fm \<Rightarrow> fm"
+definition axiom_distribimp' :: \<open>fm \<Rightarrow> fm \<Rightarrow> fm \<Rightarrow> fm\<close>
   where
-    "axiom_distribimp' p q r \<equiv> Imp (Imp p (Imp q r)) (Imp (Imp p q) (Imp p r))"
+    \<open>axiom_distribimp' p q r \<equiv> Imp (Imp p (Imp q r)) (Imp (Imp p q) (Imp p r))\<close>
 
-definition axiom_doubleneg' :: "fm \<Rightarrow> fm"
+definition axiom_doubleneg' :: \<open>fm \<Rightarrow> fm\<close>
   where
-    "axiom_doubleneg' p \<equiv> Imp (Imp (Imp p Falsity) Falsity) p"
+    \<open>axiom_doubleneg' p \<equiv> Imp (Imp (Imp p Falsity) Falsity) p\<close>
 
-definition axiom_allimp' :: "id \<Rightarrow> fm \<Rightarrow> fm \<Rightarrow> fm"
+definition axiom_allimp' :: \<open>id \<Rightarrow> fm \<Rightarrow> fm \<Rightarrow> fm\<close>
   where
-    "axiom_allimp' x p q \<equiv> Imp (Uni x (Imp p q)) (Imp (Uni x p) (Uni x q))"
+    \<open>axiom_allimp' x p q \<equiv> Imp (Uni x (Imp p q)) (Imp (Uni x p) (Uni x q))\<close>
 
-definition axiom_impall' :: "id \<Rightarrow> fm \<Rightarrow> fm"
+definition axiom_impall' :: \<open>id \<Rightarrow> fm \<Rightarrow> fm\<close>
   where
-    "axiom_impall' x p \<equiv> if \<not> free_in x p then (Imp p (Uni x p)) else fail"
+    \<open>axiom_impall' x p \<equiv> if \<not> free_in x p then (Imp p (Uni x p)) else fail\<close>
 
-definition axiom_existseq' :: "id \<Rightarrow> tm \<Rightarrow> fm"
+definition axiom_existseq' :: \<open>id \<Rightarrow> tm \<Rightarrow> fm\<close>
   where
-    "axiom_existseq' x t \<equiv> if \<not> occurs_in x t then Exi x (Pre (STR ''='') [Var x, t]) else fail"
+    \<open>axiom_existseq' x t \<equiv> if \<not> occurs_in x t then Exi x (Pre (STR ''='') [Var x, t]) else fail\<close>
 
-definition axiom_eqrefl' :: "tm \<Rightarrow> fm"
+definition axiom_eqrefl' :: \<open>tm \<Rightarrow> fm\<close>
   where
-    "axiom_eqrefl' t \<equiv> Pre (STR ''='') [t, t]"
+    \<open>axiom_eqrefl' t \<equiv> Pre (STR ''='') [t, t]\<close>
 
-definition axiom_funcong' :: "id \<Rightarrow> tm list \<Rightarrow> tm list \<Rightarrow> fm"
+definition axiom_funcong' :: \<open>id \<Rightarrow> tm list \<Rightarrow> tm list \<Rightarrow> fm\<close>
   where
-    "axiom_funcong' i l l' \<equiv> chain l l' (Pre (STR ''='') [Fun i l, Fun i l'])"
+    \<open>axiom_funcong' i l l' \<equiv> chain l l' (Pre (STR ''='') [Fun i l, Fun i l'])\<close>
 
-definition axiom_predcong' :: "id \<Rightarrow> tm list \<Rightarrow> tm list \<Rightarrow> fm"
+definition axiom_predcong' :: \<open>id \<Rightarrow> tm list \<Rightarrow> tm list \<Rightarrow> fm\<close>
   where
-    "axiom_predcong' i l l' \<equiv> chain l l' (Imp (Pre i l) (Pre i l'))"
+    \<open>axiom_predcong' i l l' \<equiv> chain l l' (Imp (Pre i l) (Pre i l'))\<close>
 
-definition axiom_iffimp1' :: "fm \<Rightarrow> fm \<Rightarrow> fm"
+definition axiom_iffimp1' :: \<open>fm \<Rightarrow> fm \<Rightarrow> fm\<close>
   where
-    "axiom_iffimp1' p q \<equiv> Imp (Iff p q) (Imp p q)"
+    \<open>axiom_iffimp1' p q \<equiv> Imp (Iff p q) (Imp p q)\<close>
 
-definition axiom_iffimp2' :: "fm \<Rightarrow> fm \<Rightarrow> fm"
+definition axiom_iffimp2' :: \<open>fm \<Rightarrow> fm \<Rightarrow> fm\<close>
   where
-    "axiom_iffimp2' p q \<equiv> Imp (Iff p q) (Imp q p)"
+    \<open>axiom_iffimp2' p q \<equiv> Imp (Iff p q) (Imp q p)\<close>
 
-definition axiom_impiff' :: "fm \<Rightarrow> fm \<Rightarrow> fm"
+definition axiom_impiff' :: \<open>fm \<Rightarrow> fm \<Rightarrow> fm\<close>
   where
-    "axiom_impiff' p q \<equiv> Imp (Imp p q) (Imp (Imp q p) (Iff p q))"
+    \<open>axiom_impiff' p q \<equiv> Imp (Imp p q) (Imp (Imp q p) (Iff p q))\<close>
 
 definition axiom_true' :: fm
   where
-    "axiom_true' \<equiv> Iff Truth (Imp Falsity Falsity)"
+    \<open>axiom_true' \<equiv> Iff Truth (Imp Falsity Falsity)\<close>
 
-definition axiom_not' :: "fm \<Rightarrow> fm"
+definition axiom_not' :: \<open>fm \<Rightarrow> fm\<close>
   where
-    "axiom_not' p \<equiv> Iff (Neg p) (Imp p Falsity)"
+    \<open>axiom_not' p \<equiv> Iff (Neg p) (Imp p Falsity)\<close>
 
-definition axiom_and' :: "fm \<Rightarrow> fm \<Rightarrow> fm"
+definition axiom_and' :: \<open>fm \<Rightarrow> fm \<Rightarrow> fm\<close>
   where
-    "axiom_and' p q \<equiv> Iff (Con p q) (Imp (Imp p (Imp q Falsity)) Falsity)"
+    \<open>axiom_and' p q \<equiv> Iff (Con p q) (Imp (Imp p (Imp q Falsity)) Falsity)\<close>
 
-definition axiom_or' :: "fm \<Rightarrow> fm \<Rightarrow> fm"
+definition axiom_or' :: \<open>fm \<Rightarrow> fm \<Rightarrow> fm\<close>
   where
-    "axiom_or' p q \<equiv> Iff (Dis p q) (Neg (Con (Neg p) (Neg q)))"
+    \<open>axiom_or' p q \<equiv> Iff (Dis p q) (Neg (Con (Neg p) (Neg q)))\<close>
 
-definition axiom_exists' :: "id \<Rightarrow> fm \<Rightarrow> fm"
+definition axiom_exists' :: \<open>id \<Rightarrow> fm \<Rightarrow> fm\<close>
   where
-    "axiom_exists' x p \<equiv> Iff (Exi x p) (Neg (Uni x (Neg p)))"
+    \<open>axiom_exists' x p \<equiv> Iff (Exi x p) (Neg (Uni x (Neg p)))\<close>
 
 section \<open>Semantics of First-Order Logic\<close>
 
-definition length2 :: "tm list \<Rightarrow> bool"
+definition length2 :: \<open>tm list \<Rightarrow> bool\<close>
   where
-    "length2 l \<equiv> case l of [_,_] \<Rightarrow> True | _ \<Rightarrow> False"
+    \<open>length2 l \<equiv> case l of [_,_] \<Rightarrow> True | _ \<Rightarrow> False\<close>
 
 primrec \<comment> \<open>Semantics of terms\<close>
-  semantics_term :: "(id \<Rightarrow> 'a) \<Rightarrow> (id \<Rightarrow> 'a list \<Rightarrow> 'a) \<Rightarrow> tm \<Rightarrow> 'a" and
-  semantics_list :: "(id \<Rightarrow> 'a) \<Rightarrow> (id \<Rightarrow> 'a list \<Rightarrow> 'a) \<Rightarrow> tm list \<Rightarrow> 'a list"
+  semantics_term :: \<open>(id \<Rightarrow> 'a) \<Rightarrow> (id \<Rightarrow> 'a list \<Rightarrow> 'a) \<Rightarrow> tm \<Rightarrow> 'a\<close> and
+  semantics_list :: \<open>(id \<Rightarrow> 'a) \<Rightarrow> (id \<Rightarrow> 'a list \<Rightarrow> 'a) \<Rightarrow> tm list \<Rightarrow> 'a list\<close>
   where
-    "semantics_term e _ (Var x) = e x" |
-    "semantics_term e f (Fun i l) = f i (semantics_list e f l)" |
-    "semantics_list _ _ [] = []" |
-    "semantics_list e f (t # l) = semantics_term e f t # semantics_list e f l"
+    \<open>semantics_term e _ (Var x) = e x\<close> |
+    \<open>semantics_term e f (Fun i l) = f i (semantics_list e f l)\<close> |
+    \<open>semantics_list _ _ [] = []\<close> |
+    \<open>semantics_list e f (t # l) = semantics_term e f t # semantics_list e f l\<close>
 
 primrec \<comment> \<open>Semantics of formulas\<close>
-  semantics :: "(id \<Rightarrow> 'a) \<Rightarrow> (id \<Rightarrow> 'a list \<Rightarrow> 'a) \<Rightarrow> (id \<Rightarrow> 'a list \<Rightarrow> bool) \<Rightarrow> fm \<Rightarrow> bool"
+  semantics :: \<open>(id \<Rightarrow> 'a) \<Rightarrow> (id \<Rightarrow> 'a list \<Rightarrow> 'a) \<Rightarrow> (id \<Rightarrow> 'a list \<Rightarrow> bool) \<Rightarrow> fm \<Rightarrow> bool\<close>
   where
-    "semantics _ _ _ Truth = True" |
-    "semantics _ _ _ Falsity = False" |
-    "semantics e f g (Pre i l) = (if i = STR ''='' \<and> length2 l
+    \<open>semantics _ _ _ Truth = True\<close> |
+    \<open>semantics _ _ _ Falsity = False\<close> |
+    \<open>semantics e f g (Pre i l) = (if i = STR ''='' \<and> length2 l
       then (semantics_term e f (hd l) = semantics_term e f (hd (tl l)))
-      else g i (semantics_list e f l))" |
-    "semantics e f g (Imp p q) = (semantics e f g p \<longrightarrow> semantics e f g q)" |
-    "semantics e f g (Iff p q) = (semantics e f g p \<longleftrightarrow> semantics e f g q)" |
-    "semantics e f g (Con p q) = (semantics e f g p \<and> semantics e f g q)" |
-    "semantics e f g (Dis p q) = (semantics e f g p \<or> semantics e f g q)" |
-    "semantics e f g (Neg p) = (\<not> semantics e f g p)" |
-    "semantics e f g (Exi x p) = (\<exists>v. semantics (e(x := v)) f g p)" |
-    "semantics e f g (Uni x p) = (\<forall>v. semantics (e(x := v)) f g p)"
+      else g i (semantics_list e f l))\<close> |
+    \<open>semantics e f g (Imp p q) = (semantics e f g p \<longrightarrow> semantics e f g q)\<close> |
+    \<open>semantics e f g (Iff p q) = (semantics e f g p \<longleftrightarrow> semantics e f g q)\<close> |
+    \<open>semantics e f g (Con p q) = (semantics e f g p \<and> semantics e f g q)\<close> |
+    \<open>semantics e f g (Dis p q) = (semantics e f g p \<or> semantics e f g q)\<close> |
+    \<open>semantics e f g (Neg p) = (\<not> semantics e f g p)\<close> |
+    \<open>semantics e f g (Exi x p) = (\<exists>v. semantics (e(x := v)) f g p)\<close> |
+    \<open>semantics e f g (Uni x p) = (\<forall>v. semantics (e(x := v)) f g p)\<close>
 
 section \<open>Definition of Proof System\<close>
 
-inductive OK :: "fm \<Rightarrow> bool" ("\<turnstile> _" 0)
+inductive OK :: \<open>fm \<Rightarrow> bool\<close> ("\<turnstile> _" 0)
   where
-    "\<turnstile> s \<Longrightarrow> \<turnstile> s' \<Longrightarrow> \<turnstile> modusponens' s s'" |
-    "\<turnstile> s \<Longrightarrow> \<turnstile> gen' _ s" |
-    "\<turnstile> axiom_addimp' _ _" |
-    "\<turnstile> axiom_distribimp' _ _ _" |
-    "\<turnstile> axiom_doubleneg' _" |
-    "\<turnstile> axiom_allimp' _ _ _" |
-    "\<turnstile> axiom_impall' _ _" |
-    "\<turnstile> axiom_existseq' _ _" |
-    "\<turnstile> axiom_eqrefl' _" |
-    "\<turnstile> axiom_funcong' _ _ _" |
-    "\<turnstile> axiom_predcong' _ _ _" |
-    "\<turnstile> axiom_iffimp1' _ _" |
-    "\<turnstile> axiom_iffimp2' _ _" |
-    "\<turnstile> axiom_impiff' _ _" |
-    "\<turnstile> axiom_true'" |
-    "\<turnstile> axiom_not' _" |
-    "\<turnstile> axiom_and' _ _" |
-    "\<turnstile> axiom_or' _ _" |
-    "\<turnstile> axiom_exists' _ _"
+    \<open>\<turnstile> s \<Longrightarrow> \<turnstile> s' \<Longrightarrow> \<turnstile> modusponens' s s'\<close> |
+    \<open>\<turnstile> s \<Longrightarrow> \<turnstile> gen' _ s\<close> |
+    \<open>\<turnstile> axiom_addimp' _ _\<close> |
+    \<open>\<turnstile> axiom_distribimp' _ _ _\<close> |
+    \<open>\<turnstile> axiom_doubleneg' _\<close> |
+    \<open>\<turnstile> axiom_allimp' _ _ _\<close> |
+    \<open>\<turnstile> axiom_impall' _ _\<close> |
+    \<open>\<turnstile> axiom_existseq' _ _\<close> |
+    \<open>\<turnstile> axiom_eqrefl' _\<close> |
+    \<open>\<turnstile> axiom_funcong' _ _ _\<close> |
+    \<open>\<turnstile> axiom_predcong' _ _ _\<close> |
+    \<open>\<turnstile> axiom_iffimp1' _ _\<close> |
+    \<open>\<turnstile> axiom_iffimp2' _ _\<close> |
+    \<open>\<turnstile> axiom_impiff' _ _\<close> |
+    \<open>\<turnstile> axiom_true'\<close> |
+    \<open>\<turnstile> axiom_not' _\<close> |
+    \<open>\<turnstile> axiom_and' _ _\<close> |
+    \<open>\<turnstile> axiom_or' _ _\<close> |
+    \<open>\<turnstile> axiom_exists' _ _\<close>
 
-proposition "\<turnstile> Imp p p"
+proposition \<open>\<turnstile> Imp p p\<close>
 proof -
-  have 1: "\<turnstile> Imp (Imp p (Imp (Imp p p) p)) (Imp (Imp p (Imp p p)) (Imp p p))"
+  have 1: \<open>\<turnstile> Imp (Imp p (Imp (Imp p p) p)) (Imp (Imp p (Imp p p)) (Imp p p))\<close>
     using OK.intros
     unfolding axiom_distribimp'_def
     by simp
 
-  have 2: "\<turnstile> Imp p (Imp (Imp p p) p)"
+  have 2: \<open>\<turnstile> Imp p (Imp (Imp p p) p)\<close>
     using OK.intros
     unfolding axiom_addimp'_def
     by simp
 
-  have 3: "\<turnstile> Imp (Imp p (Imp p p)) (Imp p p)"
+  have 3: \<open>\<turnstile> Imp (Imp p (Imp p p)) (Imp p p)\<close>
     using 1 2 OK.intros(1)
     unfolding modusponens'_def
     by fastforce
 
-  have 4: "\<turnstile> Imp p (Imp p p)"
+  have 4: \<open>\<turnstile> Imp p (Imp p p)\<close>
     using OK.intros
     unfolding axiom_addimp'_def
     by simp
 
-  have 5: "\<turnstile> Imp p p"
+  have 5: \<open>\<turnstile> Imp p p\<close>
     using 3 4 OK.intros(1)
     unfolding modusponens'_def
     by fastforce
@@ -217,35 +217,35 @@ qed
 section \<open>Soundness of Proof System\<close>
 
 lemma map':
-  "\<not> occurs_in x t \<Longrightarrow> semantics_term e f t = semantics_term (e(x := v)) f t"
-  "\<not> occurs_in_list x l \<Longrightarrow> semantics_list e f l = semantics_list (e(x := v)) f l"
+  \<open>\<not> occurs_in x t \<Longrightarrow> semantics_term e f t = semantics_term (e(x := v)) f t\<close>
+  \<open>\<not> occurs_in_list x l \<Longrightarrow> semantics_list e f l = semantics_list (e(x := v)) f l\<close>
   by (induct t and l rule: semantics_term.induct semantics_list.induct) simp_all
 
 lemma map:
-  "\<not> free_in x p \<Longrightarrow> semantics e f g p \<longleftrightarrow> semantics (e(x := v)) f g p"
+  \<open>\<not> free_in x p \<Longrightarrow> semantics e f g p \<longleftrightarrow> semantics (e(x := v)) f g p\<close>
 proof (induct p arbitrary: e)
   fix e
-  show "\<not> free_in x Truth \<Longrightarrow> semantics e f g Truth \<longleftrightarrow> semantics (e(x := v)) f g Truth"
+  show \<open>\<not> free_in x Truth \<Longrightarrow> semantics e f g Truth \<longleftrightarrow> semantics (e(x := v)) f g Truth\<close>
     by simp
 next
   fix e
-  show "\<not> free_in x Falsity \<Longrightarrow> semantics e f g Falsity \<longleftrightarrow> semantics (e(x := v)) f g Falsity"
+  show \<open>\<not> free_in x Falsity \<Longrightarrow> semantics e f g Falsity \<longleftrightarrow> semantics (e(x := v)) f g Falsity\<close>
     by simp
 next
   fix e i l
-  show "\<not> free_in x (Pre i l) \<Longrightarrow> semantics e f g (Pre i l) \<longleftrightarrow> semantics (e(x := v)) f g (Pre i l)"
+  show \<open>\<not> free_in x (Pre i l) \<Longrightarrow> semantics e f g (Pre i l) \<longleftrightarrow> semantics (e(x := v)) f g (Pre i l)\<close>
   proof -
-    assume assm: "\<not> free_in x (Pre i l)"
-    then have fresh: "\<not> occurs_in_list x l"
+    assume assm: \<open>\<not> free_in x (Pre i l)\<close>
+    then have fresh: \<open>\<not> occurs_in_list x l\<close>
       by simp
-    show "semantics e f g (Pre i l) \<longleftrightarrow> semantics (e(x := v)) f g (Pre i l)"
+    show \<open>semantics e f g (Pre i l) \<longleftrightarrow> semantics (e(x := v)) f g (Pre i l)\<close>
     proof cases
-      assume eq: "i = STR ''='' \<and> length2 l"
-      then have "semantics e f g (Pre i l) \<longleftrightarrow>
-          semantics_term e f (hd l) = semantics_term e f (hd (tl l))"
+      assume eq: \<open>i = STR ''='' \<and> length2 l\<close>
+      then have \<open>semantics e f g (Pre i l) \<longleftrightarrow>
+          semantics_term e f (hd l) = semantics_term e f (hd (tl l))\<close>
         by simp
-      also have "... \<longleftrightarrow>
-          semantics_term (e(x := v)) f (hd l) = semantics_term (e(x := v)) f (hd (tl l))"
+      also have \<open>... \<longleftrightarrow>
+          semantics_term (e(x := v)) f (hd l) = semantics_term (e(x := v)) f (hd (tl l))\<close>
         using map'(1) fresh occurs_in_list.simps(2) eq list.case_eq_if list.collapse
         unfolding length2_def
         by metis
@@ -253,10 +253,10 @@ next
         using eq
         by simp
     next
-      assume not_eq: "\<not> (i = STR ''='' \<and> length2 l)"
-      then have "semantics e f g (Pre i l) \<longleftrightarrow> g i (semantics_list e f l)"
+      assume not_eq: \<open>\<not> (i = STR ''='' \<and> length2 l)\<close>
+      then have \<open>semantics e f g (Pre i l) \<longleftrightarrow> g i (semantics_list e f l)\<close>
         by simp iprover
-      also have "... \<longleftrightarrow> g i (semantics_list (e(x := v)) f l)"
+      also have \<open>... \<longleftrightarrow> g i (semantics_list (e(x := v)) f l)\<close>
         using map'(2) fresh
         by metis
       finally show ?thesis
@@ -266,59 +266,59 @@ next
   qed
 next
   fix p1 p2 e
-  assume assm1: "\<not> free_in x p1 \<Longrightarrow> semantics e f g p1 \<longleftrightarrow> semantics (e(x := v)) f g p1" for e
-  assume assm2: "\<not> free_in x p2 \<Longrightarrow> semantics e f g p2 \<longleftrightarrow> semantics (e(x := v)) f g p2" for e
-  show "\<not> free_in x (Imp p1 p2) \<Longrightarrow>
-      semantics e f g (Imp p1 p2) \<longleftrightarrow> semantics (e(x := v)) f g (Imp p1 p2)"
+  assume assm1: \<open>\<not> free_in x p1 \<Longrightarrow> semantics e f g p1 \<longleftrightarrow> semantics (e(x := v)) f g p1\<close> for e
+  assume assm2: \<open>\<not> free_in x p2 \<Longrightarrow> semantics e f g p2 \<longleftrightarrow> semantics (e(x := v)) f g p2\<close> for e
+  show \<open>\<not> free_in x (Imp p1 p2) \<Longrightarrow>
+      semantics e f g (Imp p1 p2) \<longleftrightarrow> semantics (e(x := v)) f g (Imp p1 p2)\<close>
     using assm1 assm2
     by simp
 next
   fix p1 p2 e
-  assume assm1: "\<not> free_in x p1 \<Longrightarrow> semantics e f g p1 \<longleftrightarrow> semantics (e(x := v)) f g p1" for e
-  assume assm2: "\<not> free_in x p2 \<Longrightarrow> semantics e f g p2 \<longleftrightarrow> semantics (e(x := v)) f g p2" for e
-  show "\<not> free_in x (Iff p1 p2) \<Longrightarrow>
-      semantics e f g (Iff p1 p2) \<longleftrightarrow> semantics (e(x := v)) f g (Iff p1 p2)"
+  assume assm1: \<open>\<not> free_in x p1 \<Longrightarrow> semantics e f g p1 \<longleftrightarrow> semantics (e(x := v)) f g p1\<close> for e
+  assume assm2: \<open>\<not> free_in x p2 \<Longrightarrow> semantics e f g p2 \<longleftrightarrow> semantics (e(x := v)) f g p2\<close> for e
+  show \<open>\<not> free_in x (Iff p1 p2) \<Longrightarrow>
+      semantics e f g (Iff p1 p2) \<longleftrightarrow> semantics (e(x := v)) f g (Iff p1 p2)\<close>
     using assm1 assm2
     by simp
 next
   fix p1 p2 e
-  assume assm1: "\<not> free_in x p1 \<Longrightarrow> semantics e f g p1 \<longleftrightarrow> semantics (e(x := v)) f g p1" for e
-  assume assm2: "\<not> free_in x p2 \<Longrightarrow> semantics e f g p2 \<longleftrightarrow> semantics (e(x := v)) f g p2" for e
-  show "\<not> free_in x (Con p1 p2) \<Longrightarrow>
-      semantics e f g (Con p1 p2) \<longleftrightarrow> semantics (e(x := v)) f g (Con p1 p2)"
+  assume assm1: \<open>\<not> free_in x p1 \<Longrightarrow> semantics e f g p1 \<longleftrightarrow> semantics (e(x := v)) f g p1\<close> for e
+  assume assm2: \<open>\<not> free_in x p2 \<Longrightarrow> semantics e f g p2 \<longleftrightarrow> semantics (e(x := v)) f g p2\<close> for e
+  show \<open>\<not> free_in x (Con p1 p2) \<Longrightarrow>
+      semantics e f g (Con p1 p2) \<longleftrightarrow> semantics (e(x := v)) f g (Con p1 p2)\<close>
     using assm1 assm2
     by simp
 next
   fix p1 p2 e
-  assume assm1: "\<not> free_in x p1 \<Longrightarrow> semantics e f g p1 \<longleftrightarrow> semantics (e(x := v)) f g p1" for e
-  assume assm2: "\<not> free_in x p2 \<Longrightarrow> semantics e f g p2 \<longleftrightarrow> semantics (e(x := v)) f g p2" for e
-  show "\<not> free_in x (Dis p1 p2) \<Longrightarrow>
-      semantics e f g (Dis p1 p2) \<longleftrightarrow> semantics (e(x := v)) f g (Dis p1 p2)"
+  assume assm1: \<open>\<not> free_in x p1 \<Longrightarrow> semantics e f g p1 \<longleftrightarrow> semantics (e(x := v)) f g p1\<close> for e
+  assume assm2: \<open>\<not> free_in x p2 \<Longrightarrow> semantics e f g p2 \<longleftrightarrow> semantics (e(x := v)) f g p2\<close> for e
+  show \<open>\<not> free_in x (Dis p1 p2) \<Longrightarrow>
+      semantics e f g (Dis p1 p2) \<longleftrightarrow> semantics (e(x := v)) f g (Dis p1 p2)\<close>
     using assm1 assm2
     by simp
 next
   fix p e
-  assume "\<not> free_in x p \<Longrightarrow> semantics e f g p \<longleftrightarrow> semantics (e(x := v)) f g p" for e
-  then show "\<not> free_in x (Neg p) \<Longrightarrow> semantics e f g (Neg p) \<longleftrightarrow> semantics (e(x := v)) f g (Neg p)"
+  assume \<open>\<not> free_in x p \<Longrightarrow> semantics e f g p \<longleftrightarrow> semantics (e(x := v)) f g p\<close> for e
+  then show \<open>\<not> free_in x (Neg p) \<Longrightarrow> semantics e f g (Neg p) \<longleftrightarrow> semantics (e(x := v)) f g (Neg p)\<close>
     by simp
 next
   fix x1 p e
-  assume "\<not> free_in x p \<Longrightarrow> semantics e f g p \<longleftrightarrow> semantics (e(x := v)) f g p" for e
-  then show "\<not> free_in x (Exi x1 p) \<Longrightarrow>
-      semantics e f g (Exi x1 p) \<longleftrightarrow> semantics (e(x := v)) f g (Exi x1 p)"
+  assume \<open>\<not> free_in x p \<Longrightarrow> semantics e f g p \<longleftrightarrow> semantics (e(x := v)) f g p\<close> for e
+  then show \<open>\<not> free_in x (Exi x1 p) \<Longrightarrow>
+      semantics e f g (Exi x1 p) \<longleftrightarrow> semantics (e(x := v)) f g (Exi x1 p)\<close>
     by simp (metis fun_upd_twist fun_upd_upd)
 next
   fix x1 p e
-  assume "\<not> free_in x p \<Longrightarrow> semantics e f g p \<longleftrightarrow> semantics (e(x := v)) f g p" for e
-  then show "\<not> free_in x (Uni x1 p) \<Longrightarrow>
-      semantics e f g (Uni x1 p) \<longleftrightarrow> semantics (e(x := v)) f g (Uni x1 p)"
+  assume \<open>\<not> free_in x p \<Longrightarrow> semantics e f g p \<longleftrightarrow> semantics (e(x := v)) f g p\<close> for e
+  then show \<open>\<not> free_in x (Uni x1 p) \<Longrightarrow>
+      semantics e f g (Uni x1 p) \<longleftrightarrow> semantics (e(x := v)) f g (Uni x1 p)\<close>
     by simp (metis fun_upd_twist fun_upd_upd)
 qed
 
 lemma length2_equiv:
-  "length2 l \<longleftrightarrow> [hd l, hd (tl l)] = l"
+  \<open>length2 l \<longleftrightarrow> [hd l, hd (tl l)] = l\<close>
 proof -
-  have "length2 l \<Longrightarrow> [hd l, hd (tl l)] = l"
+  have \<open>length2 l \<Longrightarrow> [hd l, hd (tl l)] = l\<close>
     unfolding length2_def
     using list.case_eq_if list.exhaust_sel
     by metis
@@ -329,31 +329,31 @@ proof -
 qed
 
 lemma equal_length_sym:
-  "equal_length l l' \<Longrightarrow> equal_length l' l"
+  \<open>equal_length l l' \<Longrightarrow> equal_length l' l\<close>
 proof (induct l' arbitrary: l)
   fix l
-  assume "equal_length l []"
-  then show "equal_length [] l"
+  assume \<open>equal_length l []\<close>
+  then show \<open>equal_length [] l\<close>
     using equal_length.simps list.case_eq_if
     by metis
 next
   fix l l' a
-  assume sym: "equal_length l l' \<Longrightarrow> equal_length l' l" for l
-  assume "equal_length l (a # l')"
-  then show "equal_length (a # l') l"
+  assume sym: \<open>equal_length l l' \<Longrightarrow> equal_length l' l\<close> for l
+  assume \<open>equal_length l (a # l')\<close>
+  then show \<open>equal_length (a # l') l\<close>
     using equal_length.simps list.case_eq_if list.collapse list.inject sym
     by metis
 qed
 
 lemma equal_length2:
-  "equal_length l l' \<Longrightarrow> length2 l \<longleftrightarrow> length2 l'"
+  \<open>equal_length l l' \<Longrightarrow> length2 l \<longleftrightarrow> length2 l'\<close>
 proof -
-  assume assm: "equal_length l l'"
-  have "equal_length l [t, t'] \<Longrightarrow> length2 l" for t t'
+  assume assm: \<open>equal_length l l'\<close>
+  have \<open>equal_length l [t, t'] \<Longrightarrow> length2 l\<close> for t t'
     unfolding length2_def
     using equal_length.simps list.case_eq_if
     by metis
-  moreover have "equal_length [t, t'] l' \<Longrightarrow> length2 l'" for t t'
+  moreover have \<open>equal_length [t, t'] l' \<Longrightarrow> length2 l'\<close> for t t'
     unfolding length2_def
     using equal_length.simps list.case_eq_if equal_length_sym
     by metis
@@ -363,18 +363,18 @@ proof -
 qed
 
 lemma imp_chain_equiv:
-  "semantics e f g (foldr Imp l p) \<longleftrightarrow> (\<forall>q \<in> set l. semantics e f g q) \<longrightarrow> semantics e f g p"
+  \<open>semantics e f g (foldr Imp l p) \<longleftrightarrow> (\<forall>q \<in> set l. semantics e f g q) \<longrightarrow> semantics e f g p\<close>
   using imp_conjL
   by (induct l) simp_all
 
 lemma imp_chain_zip_eq:
-  "equal_length l l' \<Longrightarrow>
+  \<open>equal_length l l' \<Longrightarrow>
       semantics e f g (foldr Imp (zip_eq l l') p) \<longleftrightarrow>
-      semantics_list e f l = semantics_list e f l' \<longrightarrow> semantics e f g p"
+      semantics_list e f l = semantics_list e f l' \<longrightarrow> semantics e f g p\<close>
 proof -
-  assume "equal_length l l'"
-  then have "(\<forall>q \<in> set (zip_eq l l'). semantics e f g q) \<longleftrightarrow>
-      semantics_list e f l = semantics_list e f l'"
+  assume \<open>equal_length l l'\<close>
+  then have \<open>(\<forall>q \<in> set (zip_eq l l'). semantics e f g q) \<longleftrightarrow>
+      semantics_list e f l = semantics_list e f l'\<close>
     unfolding zip_eq_def
     using length2_def
     by (induct l l' rule: list_induct2') simp_all
@@ -384,21 +384,21 @@ proof -
 qed
 
 lemma funcong:
-  "equal_length l l' \<Longrightarrow>
-      semantics e f g (foldr Imp (zip_eq l l') (Pre (STR ''='') [Fun i l, Fun i l']))"
+  \<open>equal_length l l' \<Longrightarrow>
+      semantics e f g (foldr Imp (zip_eq l l') (Pre (STR ''='') [Fun i l, Fun i l']))\<close>
 proof -
-  assume assm: "equal_length l l'"
+  assume assm: \<open>equal_length l l'\<close>
   show ?thesis
   proof cases
-    assume "semantics_list e f l = semantics_list e f l'"
-    then have "semantics e f g (Pre (STR ''='') [Fun i l, Fun i l'])"
+    assume \<open>semantics_list e f l = semantics_list e f l'\<close>
+    then have \<open>semantics e f g (Pre (STR ''='') [Fun i l, Fun i l'])\<close>
       using length2_def
       by simp
     then show ?thesis
       using imp_chain_equiv
       by iprover
   next
-    assume "semantics_list e f l \<noteq> semantics_list e f l'"
+    assume \<open>semantics_list e f l \<noteq> semantics_list e f l'\<close>
     then show ?thesis
       using assm imp_chain_zip_eq
       by iprover
@@ -406,44 +406,44 @@ proof -
 qed
 
 lemma predcong:
-  "equal_length l l' \<Longrightarrow>
-      semantics e f g (foldr Imp (zip_eq l l') (Imp (Pre i l) (Pre i l')))"
+  \<open>equal_length l l' \<Longrightarrow>
+      semantics e f g (foldr Imp (zip_eq l l') (Imp (Pre i l) (Pre i l')))\<close>
 proof -
-  assume assm: "equal_length l l'"
+  assume assm: \<open>equal_length l l'\<close>
   show ?thesis
   proof cases
-    assume eq: "i = STR ''='' \<and> length2 l \<and> length2 l'"
+    assume eq: \<open>i = STR ''='' \<and> length2 l \<and> length2 l'\<close>
     show ?thesis
     proof cases
-      assume "semantics_list e f l = semantics_list e f l'"
-      then have "semantics_list e f [hd l, hd (tl l)] = semantics_list e f [hd l', hd (tl l')]"
+      assume \<open>semantics_list e f l = semantics_list e f l'\<close>
+      then have \<open>semantics_list e f [hd l, hd (tl l)] = semantics_list e f [hd l', hd (tl l')]\<close>
         using eq length2_equiv
         by simp
-      then have "semantics e f g (Imp (Pre (STR ''='') l) (Pre (STR ''='') l'))"
+      then have \<open>semantics e f g (Imp (Pre (STR ''='') l) (Pre (STR ''='') l'))\<close>
         using eq
         by simp
       then show ?thesis
         using eq imp_chain_equiv
         by iprover
     next
-      assume "semantics_list e f l \<noteq> semantics_list e f l'"
+      assume \<open>semantics_list e f l \<noteq> semantics_list e f l'\<close>
       then show ?thesis
         using assm imp_chain_zip_eq
         by iprover
     qed
   next
-    assume not_eq: "\<not> (i = STR ''='' \<and> length2 l \<and> length2 l')"
+    assume not_eq: \<open>\<not> (i = STR ''='' \<and> length2 l \<and> length2 l')\<close>
     show ?thesis
     proof cases
-      assume "semantics_list e f l = semantics_list e f l'"
-      then have "semantics e f g (Imp (Pre i l) (Pre i l'))"
+      assume \<open>semantics_list e f l = semantics_list e f l'\<close>
+      then have \<open>semantics e f g (Imp (Pre i l) (Pre i l'))\<close>
         using assm not_eq equal_length2
         by simp iprover
       then show ?thesis
         using imp_chain_equiv
         by iprover
     next
-      assume "semantics_list e f l \<noteq> semantics_list e f l'"
+      assume \<open>semantics_list e f l \<noteq> semantics_list e f l'\<close>
       then show ?thesis
         using assm imp_chain_zip_eq
         by iprover
@@ -452,196 +452,196 @@ proof -
 qed
 
 theorem soundness':
-  "\<turnstile> p \<Longrightarrow> semantics e f g p"
+  \<open>\<turnstile> p \<Longrightarrow> semantics e f g p\<close>
 proof (induct arbitrary: e rule: OK.induct)
   fix e s s'
-  assume "semantics e f g s" "semantics e f g s'" for e
-  then show "semantics e f g (modusponens' s s')"
+  assume \<open>semantics e f g s\<close> \<open>semantics e f g s'\<close> for e
+  then show \<open>semantics e f g (modusponens' s s')\<close>
     unfolding modusponens'_def
     by (cases s) simp_all
 next
   fix e x s
-  assume "semantics e f g s" for e
-  then show "semantics e f g (gen' x s)"
+  assume \<open>semantics e f g s\<close> for e
+  then show \<open>semantics e f g (gen' x s)\<close>
     unfolding gen'_def
     by simp
 next
   fix e p q
-  show "semantics e f g (axiom_addimp' p q)"
+  show \<open>semantics e f g (axiom_addimp' p q)\<close>
     unfolding axiom_addimp'_def
     by simp
 next
   fix e p q r
-  show "semantics e f g (axiom_distribimp' p q r)"
+  show \<open>semantics e f g (axiom_distribimp' p q r)\<close>
     unfolding axiom_distribimp'_def
     by simp
 next
   fix e g p
-  show "semantics e f g (axiom_doubleneg' p)"
+  show \<open>semantics e f g (axiom_doubleneg' p)\<close>
     unfolding axiom_doubleneg'_def
     by simp
 next
   fix e x p q
-  show "semantics e f g (axiom_allimp' x p q)"
+  show \<open>semantics e f g (axiom_allimp' x p q)\<close>
     unfolding axiom_allimp'_def
     by simp
 next
   fix e x p
-  show "semantics e f g (axiom_impall' x p)"
+  show \<open>semantics e f g (axiom_impall' x p)\<close>
     unfolding axiom_impall'_def
     using map
     by simp iprover
 next
   fix e x t
-  show "semantics e f g (axiom_existseq' x t)"
+  show \<open>semantics e f g (axiom_existseq' x t)\<close>
     unfolding axiom_existseq'_def
     using map'(1) length2_def
     by simp iprover
 next
   fix e t
-  show "semantics e f g (axiom_eqrefl' t)"
+  show \<open>semantics e f g (axiom_eqrefl' t)\<close>
     unfolding axiom_eqrefl'_def
     using length2_def
     by simp
 next
   fix e i l l'
-  show "semantics e f g (axiom_funcong' i l l')"
+  show \<open>semantics e f g (axiom_funcong' i l l')\<close>
     unfolding axiom_funcong'_def
     using funcong
     by simp standard
 next
   fix e i l l'
-  show "semantics e f g (axiom_predcong' i l l')"
+  show \<open>semantics e f g (axiom_predcong' i l l')\<close>
     unfolding axiom_predcong'_def
     using predcong
     by simp standard
 next
   fix e p q
-  show "semantics e f g (axiom_iffimp1' p q)"
+  show \<open>semantics e f g (axiom_iffimp1' p q)\<close>
     unfolding axiom_iffimp1'_def
     by simp
 next
   fix e p q
-  show "semantics e f g (axiom_iffimp2' p q)"
+  show \<open>semantics e f g (axiom_iffimp2' p q)\<close>
     unfolding axiom_iffimp2'_def
     by simp
 next
   fix e p q
-  show "semantics e f g (axiom_impiff' p q)"
+  show \<open>semantics e f g (axiom_impiff' p q)\<close>
     unfolding axiom_impiff'_def
     by simp (rule impI, rule impI, rule iffI, erule mp, assumption, erule mp, assumption)
 next
   fix e
-  show "semantics e f g (axiom_true')"
+  show \<open>semantics e f g (axiom_true')\<close>
     unfolding axiom_true'_def
     by simp
 next
   fix e p
-  show "semantics e f g (axiom_not' p)"
+  show \<open>semantics e f g (axiom_not' p)\<close>
     unfolding axiom_not'_def
     by simp
 next
   fix e p q
-  show "semantics e f g (axiom_and' p q)"
+  show \<open>semantics e f g (axiom_and' p q)\<close>
     unfolding axiom_and'_def
     by simp
 next
   fix e p q
-  show "semantics e f g (axiom_or' p q)"
+  show \<open>semantics e f g (axiom_or' p q)\<close>
     unfolding axiom_or'_def
     by simp
 next
   fix e x p
-  show "semantics e f g (axiom_exists' x p)"
+  show \<open>semantics e f g (axiom_exists' x p)\<close>
     unfolding axiom_exists'_def
     by simp
 qed
 
-corollary consistency': "\<not> (\<turnstile> Falsity)"
+corollary consistency': \<open>\<not> (\<turnstile> Falsity)\<close>
   using soundness'
   by fastforce
 
 section \<open>Definition of Theorems as a Type\<close>
 
-typedef "thm" = "{p :: fm. \<turnstile> p}"
+typedef "thm" = \<open>{p :: fm. \<turnstile> p}\<close>
 proof -
-  have "\<turnstile> axiom_addimp' Truth Truth"
+  have \<open>\<turnstile> axiom_addimp' Truth Truth\<close>
     using OK.intros by auto
   then show ?thesis by blast
 qed
 
-definition "concl \<equiv> Rep_thm"
+definition \<open>concl \<equiv> Rep_thm\<close>
 declare concl_def[simp]
 
 setup_lifting type_definition_thm
 
 section \<open>Soundness of Proof System as a Type\<close>
 
-theorem soundness: "semantics e f g (concl p)"
+theorem soundness: \<open>semantics e f g (concl p)\<close>
   using soundness' Rep_thm
   by fastforce
 
-theorem consistency: "concl p \<noteq> Falsity"
+theorem consistency: \<open>concl p \<noteq> Falsity\<close>
   using consistency' Rep_thm concl_def mem_Collect_eq
   by metis
 
 section \<open>Definition of Rules and Axioms on Theorems\<close>
 
-lift_definition modusponens :: "thm \<Rightarrow> thm \<Rightarrow> thm" is modusponens'
+lift_definition modusponens :: \<open>thm \<Rightarrow> thm \<Rightarrow> thm\<close> is modusponens'
   using OK.intros(1) .
 
-lift_definition gen :: "id \<Rightarrow> thm \<Rightarrow> thm" is gen'
+lift_definition gen :: \<open>id \<Rightarrow> thm \<Rightarrow> thm\<close> is gen'
   using OK.intros(2) .
 
-lift_definition axiom_addimp :: "fm \<Rightarrow> fm \<Rightarrow> thm" is axiom_addimp'
+lift_definition axiom_addimp :: \<open>fm \<Rightarrow> fm \<Rightarrow> thm\<close> is axiom_addimp'
   using OK.intros(3) .
 
-lift_definition axiom_distribimp :: "fm \<Rightarrow> fm \<Rightarrow> fm \<Rightarrow> thm" is axiom_distribimp'
+lift_definition axiom_distribimp :: \<open>fm \<Rightarrow> fm \<Rightarrow> fm \<Rightarrow> thm\<close> is axiom_distribimp'
   using OK.intros(4) .
 
-lift_definition axiom_doubleneg :: "fm \<Rightarrow> thm" is axiom_doubleneg'
+lift_definition axiom_doubleneg :: \<open>fm \<Rightarrow> thm\<close> is axiom_doubleneg'
   using OK.intros(5) .
 
-lift_definition axiom_allimp :: "id \<Rightarrow> fm \<Rightarrow> fm \<Rightarrow> thm" is axiom_allimp'
+lift_definition axiom_allimp :: \<open>id \<Rightarrow> fm \<Rightarrow> fm \<Rightarrow> thm\<close> is axiom_allimp'
   using OK.intros(6) .
 
-lift_definition axiom_impall :: "id \<Rightarrow> fm \<Rightarrow> thm" is axiom_impall'
+lift_definition axiom_impall :: \<open>id \<Rightarrow> fm \<Rightarrow> thm\<close> is axiom_impall'
   using OK.intros(7) .
 
-lift_definition axiom_existseq :: "id \<Rightarrow> tm \<Rightarrow> thm" is axiom_existseq'
+lift_definition axiom_existseq :: \<open>id \<Rightarrow> tm \<Rightarrow> thm\<close> is axiom_existseq'
   using OK.intros(8) .
 
-lift_definition axiom_eqrefl :: "tm \<Rightarrow> thm" is axiom_eqrefl'
+lift_definition axiom_eqrefl :: \<open>tm \<Rightarrow> thm\<close> is axiom_eqrefl'
   using OK.intros(9) .
 
-lift_definition axiom_funcong :: "id \<Rightarrow> tm list \<Rightarrow> tm list \<Rightarrow> thm" is axiom_funcong'
+lift_definition axiom_funcong :: \<open>id \<Rightarrow> tm list \<Rightarrow> tm list \<Rightarrow> thm\<close> is axiom_funcong'
   using OK.intros(10) .
 
-lift_definition axiom_predcong :: "id \<Rightarrow> tm list \<Rightarrow> tm list \<Rightarrow> thm" is axiom_predcong'
+lift_definition axiom_predcong :: \<open>id \<Rightarrow> tm list \<Rightarrow> tm list \<Rightarrow> thm\<close> is axiom_predcong'
   using OK.intros(11) .
 
-lift_definition axiom_iffimp1 :: "fm \<Rightarrow> fm \<Rightarrow> thm" is axiom_iffimp1'
+lift_definition axiom_iffimp1 :: \<open>fm \<Rightarrow> fm \<Rightarrow> thm\<close> is axiom_iffimp1'
   using OK.intros(12) .
 
-lift_definition axiom_iffimp2 :: "fm \<Rightarrow> fm \<Rightarrow> thm" is axiom_iffimp2'
+lift_definition axiom_iffimp2 :: \<open>fm \<Rightarrow> fm \<Rightarrow> thm\<close> is axiom_iffimp2'
   using OK.intros(13) .
 
-lift_definition axiom_impiff :: "fm \<Rightarrow> fm \<Rightarrow> thm" is axiom_impiff'
+lift_definition axiom_impiff :: \<open>fm \<Rightarrow> fm \<Rightarrow> thm\<close> is axiom_impiff'
   using OK.intros(14) .
 
-lift_definition axiom_true :: "thm" is axiom_true'
+lift_definition axiom_true :: \<open>thm\<close> is axiom_true'
   using OK.intros(15) .
 
-lift_definition axiom_not :: "fm \<Rightarrow> thm" is axiom_not'
+lift_definition axiom_not :: \<open>fm \<Rightarrow> thm\<close> is axiom_not'
   using OK.intros(16) .
 
-lift_definition axiom_and :: "fm \<Rightarrow> fm \<Rightarrow> thm" is axiom_and'
+lift_definition axiom_and :: \<open>fm \<Rightarrow> fm \<Rightarrow> thm\<close> is axiom_and'
   using OK.intros(17) .
 
-lift_definition axiom_or :: "fm \<Rightarrow> fm \<Rightarrow> thm" is axiom_or'
+lift_definition axiom_or :: \<open>fm \<Rightarrow> fm \<Rightarrow> thm\<close> is axiom_or'
   using OK.intros(18) .
 
-lift_definition axiom_exists :: "id \<Rightarrow> fm \<Rightarrow> thm" is axiom_exists'
+lift_definition axiom_exists :: \<open>id \<Rightarrow> fm \<Rightarrow> thm\<close> is axiom_exists'
   using OK.intros(19) .
 
 section \<open>ML Code Reflection\<close>
